\documentclass{article}
\usepackage{amsmath}
\begin{document}
\noindent Let $q = 1, p = 0$ and
$
T_{pq}^n:
\begin{cases}
  a_n = b_{n-1}q + a_{n-1}q + a_{n-1}p\\
  b_n = b_{n-1}p + a_{n-1}q
\end{cases}$\\
  
$\Rightarrow
T_{pq}^{n+1} :
\begin{cases}
  a_{n+1} = b_{n-1} (2pq + q^2) + a_{n-1} (q^2 + 2pq)
  + a_{n-1} (p^2 + q^2)\\
  b_{n+1} = b_{n-1}(p^2+q^2) + a_{n-1} (2pq + q^2)
  \end{cases}
  $\\
  Let $q' = 2pq + q^2 $ and $p' = p^2 + q^2$\\
  $\Rightarrow T_{pq}^n = (T_{p'q'}^{\frac{n}{2}})$
 
\end{document}