\documentclass{article}
\usepackage{amsmath}
\usepackage{amssymb}
\begin{document}
\noindent Let $ (x,y) \in \mathbb{N}^2 $, let  $ (\epsilon',\epsilon) \in [0, 1[^2 $\\
$ \implies (x + \epsilon') * (y + \epsilon) = xy + y \epsilon' + x\epsilon + \epsilon'\epsilon $\\
Given $ \epsilon' = x\alpha' $ and $\epsilon = y\alpha , (\alpha,\alpha') \in [0, 1[^2$\\
$\implies (x+\epsilon') * (y + \epsilon) = xy + xy \alpha' + xy \alpha + xy \alpha\alpha' $\\
Given $  \alpha\alpha = o(xy + xy\alpha'  + xy\alpha) $ \\
$\implies (x+\epsilon') * (y + \epsilon) \sim xy + xy (\alpha + \alpha') \blacksquare$


\end{document} 
